Refactor of Reg.v. Added Util.v

theories/Reg.v
@@ -3,51 +3,145 @@
     "A Play on Regular Expressions" — Fischer, Huch, and Wilke (ICFP 2010).
 *)
 
-From Stdlib Require Import String List Ascii Nat Program.Wf Lia.
+From Stdlib Require Import List Lia Program.Equality.
+From MarkedRegex Require Import Util.
 Import ListNotations.
 
+Section RegDef.
+(** * Definition of Reg
+
+    This sections defines  inductive Reg type presented in the paper *)
+
+    Context {A : Type}.
+
 (** Polymorphic regular expressions *)
-Inductive Reg (A : Type) : Type :=
-| Eps : Reg A                         (* ε *)
-| Sym : A -> Reg A                    (* a *)
-| Alt : Reg A -> Reg A -> Reg A       (* α | β *)
-| Seq : Reg A -> Reg A -> Reg A       (* α β *)
-| Rep : Reg A -> Reg A.               (* α* *)
+Inductive Reg : Type :=
+| Eps : Reg                     (* ε *)
+| Sym : A -> Reg                (* a *)
+| Alt : Reg -> Reg -> Reg       (* α | β *)
+| Seq : Reg -> Reg -> Reg       (* α β *)
+| Rep : Reg -> Reg.             (* α* *)
 
-Definition RegChar := Reg Ascii.ascii.
-Definition RegBool := Reg bool.
+End RegDef.
 
-Fixpoint language_of {A : Type} (r : Reg A) (w : list A) : Prop :=
+Section Semantics.
+  (** * Definitions of language_of
+
+    This sections defines the semantical function
+    language_of : forall (A : Type), Reg A -> list A -> Prop 
+    in two ways, first one is using Fixpoint and the other one uses Inductive *)
+
+    Context {A : Type}.
+
+Fixpoint language_of (r : Reg) (w : list A) : Prop :=
   match r with
-  | Eps _ => w = []
-  | Sym _ a => w = [a]
-  | Alt _ r1 r2 => language_of r1 w \/ language_of r2 w
-  | Seq _ r1 r2 =>
+  | Eps => w = []
+  | Sym a => w = [a]
+  | Alt r1 r2 => language_of r1 w \/ language_of r2 w
+  | Seq r1 r2 =>
       exists w1 w2,
         w = w1 ++ w2 /\
         language_of r1 w1 /\
         language_of r2 w2
-  | Rep _ r' =>
-      exists n (ws : list (list A)),
-        (* partition en n sous-mots non vides *)
-        length ws = n /\
+  | Rep r' =>
+      exists (ws : list (list A)),
         concat ws = w /\
         (forall wi, In wi ws -> language_of r' wi)
   end.
 
-(* Inductive version *)
-(* Inductive language_of {A : Type} : Reg A -> list A -> Prop :=
-| LangEps : forall w, w = [] -> language_of (Eps A) w
-| LangSym : forall a, language_of (Sym A a) [a]
-| LangAltL : forall r1 r2 w, language_of r1 w -> language_of (Alt A r1 r2) w
-| LangAltR : forall r1 r2 w, language_of r2 w -> language_of (Alt A r1 r2) w
+Inductive language_of_ind : Reg -> list A -> Prop :=
+| LangEps : forall w, w = [] -> language_of_ind Eps w
+| LangSym : forall a, language_of_ind (Sym a) [a]
+| LangAltL : forall r1 r2 w, language_of_ind r1 w -> language_of_ind (Alt r1 r2) w
+| LangAltR : forall r1 r2 w, language_of_ind r2 w -> language_of_ind (Alt r1 r2) w
 | LangSeq : forall r1 r2 w1 w2,
-    language_of r1 w1 ->
-    language_of r2 w2 ->
-    language_of (Seq A r1 r2) (w1 ++ w2)
-| LangRep0 : forall r, language_of (Rep A r) []
+    language_of_ind r1 w1 ->
+    language_of_ind r2 w2 ->
+    language_of_ind (Seq r1 r2) (w1 ++ w2)
+| LangRep0 : forall r, language_of_ind (Rep r) []
 | LangRepStep : forall r w1 w2,
-    w1 <> [] ->
-    language_of r w1 ->
-    language_of (Rep A r) w2 ->
-    language_of (Rep A r) (w1 ++ w2). *)
+    w1 <> [] -> language_of_ind r w1 ->
+    language_of_ind (Rep r) w2 ->
+    language_of_ind (Rep r) (w1 ++ w2).
+
+End Semantics.
+
+Section Equivalence.
+  (** * Equivalence of these two definitions
+
+    In this section, we prove that language_of and language_of_ind are equivalent. *)
+
+    Context {A : Type}.
+
+Proposition language_of_to_ind :  
+  forall (r : Reg) (w : list A),
+    language_of r w -> language_of_ind r w.
+Proof.
+  intros r. induction r.
+  - intros. unfold language_of in H. rewrite H. apply LangEps. reflexivity.
+  - intros. unfold language_of in H. rewrite H. apply LangSym.
+  - intros. destruct H.
+    * apply LangAltL. apply IHr1. assumption.
+    * apply LangAltR. apply IHr2. assumption.
+- intros. destruct H as [l1 [l2 [concat [H H']]]].
+    apply IHr1 in H. apply IHr2 in H'. 
+    rewrite concat. apply LangSeq. 
+    assumption. assumption. 
+  - intros. destruct H as [x [H]]. rewrite <- H. clear H w. 
+  induction x.
+    * rewrite concat_nil. apply LangRep0.
+    * pose proof ((IHr a) ((H0 a) (in_eq a x))). 
+    assert (forall wi : list A, In wi x -> language_of r wi).
+      + intros. pose proof ((H0 wi) ((in_cons a wi x) H1)). assumption.
+      + pose proof (IHx H1). clear IHx H1. destruct a.
+       -- assumption.
+       -- assert ([] <> a :: a0) as Hnil by (apply nil_cons).
+          apply ((LangRepStep r (a::a0) (concat x)) (not_eq_sym Hnil) H H2).
+Qed.
+
+
+Lemma language_of_to_fix :
+  forall (r : Reg) (w : list A),
+    language_of_ind r w -> language_of r w.
+Proof.
+  intros r. induction r. 
+  - intros. dependent destruction H. assumption.
+  - intros. dependent destruction H. simpl. reflexivity.
+  - intros. dependent destruction H. simpl. 
+      left.  apply ((IHr1 w) H).
+      right. apply ((IHr2 w) H).
+  - intros. dependent destruction H. simpl. exists w1. exists w2. repeat split.
+    + apply ((IHr1 w1) H).
+    + apply ((IHr2 w2) H0).
+  - intros. assert (exists (ws : list (list A)),
+        concat ws = w /\ (forall wi, In wi ws -> language_of_ind r wi)).
+  strong_induction w.
+    + exists []. split.
+      * apply concat_nil.
+      * intros. inversion H0.
+    + dependent destruction H.
+      * exists []. split.
+        -- apply concat_nil.
+        -- intros. inversion H.
+      * rewrite <- length_zero_iff_nil in H. apply not_eq_sym in H.
+        apply (Arith_base.neq_0_lt_stt (Datatypes.length w1)) in H.
+        assert (length w2 < length w1 + length w2) by lia. rewrite <- (length_app w1 w2) in H3.
+        pose proof (H0 w2 H3 H2). destruct H4. exists (w1 :: x). split.
+        -- rewrite concat_cons. destruct H4. rewrite H4. reflexivity. 
+        -- destruct H4. intros. destruct H6.
+          ++ rewrite <- H6. apply H1.
+          ++ apply (H5 wi H6).
+    + simpl. repeat destruct H0. clear H. exists x. split. reflexivity. intros. 
+    apply ((IHr wi) (H1 wi H)).
+Qed.
+
+Theorem language_of_equiv :
+  forall (r : Reg) (w : list A),
+    language_of r w <-> language_of_ind r w.
+Proof.
+  intros r w. split.
+  - apply language_of_to_ind.
+  - apply language_of_to_fix.
+Qed.
+
+End Equivalence.
